Finish missing proofs to reduce TCB

vale/code/arch/x64/X64.BufferViewStore.fsti
@@ -18,13 +18,14 @@ val bv_upd_update_heap64:
   (addrs:addr_map) ->
   (ptrs:list s8) ->
   (h:HS.mem{B.live h b}) ->
-   Lemma (
-     let bv = BV.mk_buffer_view b view64 in
+   Lemma
+     (requires correct_down_p h addrs heap b)
+     (ensures (let bv = BV.mk_buffer_view b view64 in
      BV.as_buffer_mk_buffer_view b view64;
      BV.get_view_mk_buffer_view b view64;
      BV.length_eq bv;
      let heap' = update_heap64 (addrs b + 8 `op_Multiply` i) v heap in
-     BV.upd h bv i (UInt64.uint_to_t v) == B.g_upd_seq b (get_seq_heap heap' addrs b) h)
+     BV.upd h bv i (UInt64.uint_to_t v) == B.g_upd_seq b (get_seq_heap heap' addrs b) h))
 
 val bv_upd_update_heap128:
   (b:s8{B.length b % 16 == 0}) ->
@@ -34,10 +35,11 @@ val bv_upd_update_heap128:
   (addrs:addr_map) ->
   (ptrs:list s8) ->
   (h:HS.mem{B.live h b}) ->
-   Lemma (
-     let bv = BV.mk_buffer_view b view128 in
+   Lemma 
+     (requires correct_down_p h addrs heap b)
+     (ensures (let bv = BV.mk_buffer_view b view128 in
      BV.as_buffer_mk_buffer_view b view128;
      BV.get_view_mk_buffer_view b view128;
      BV.length_eq bv;
      let heap' = update_heap128 (addrs b + 16 `op_Multiply` i) v heap in
-     BV.upd h bv i v == B.g_upd_seq b (get_seq_heap heap' addrs b) h)
+     BV.upd h bv i v == B.g_upd_seq b (get_seq_heap heap' addrs b) h))
